Veir/Benchmarks.lean
@@ -18,119 +18,119 @@ namespace Pattern
 
 def addIConstantFolding (rewriter: PatternRewriter OpCode) (op: OperationPtr) : Option (PatternRewriter OpCode) := do
   -- Check that the operation is an arith.addi operation
-  if op.getOpType rewriter.ctx sorry ≠ .arith .addi then
+  if op.getOpType rewriter.ctx.val sorry ≠ .arith .addi then
     return rewriter
 
   -- Get the lhs and check that it is a constant
-  let lhsValuePtr := op.getOperand rewriter.ctx 0 (by sorry) (by sorry)
+  let lhsValuePtr := op.getOperand rewriter.ctx.val 0 (by sorry) (by sorry)
   let lhsOp ← match lhsValuePtr with
   | ValuePtr.opResult lhsOpResultPtr => some lhsOpResultPtr.op
   | _ => none
-  let lhsOpStruct := lhsOp.get rewriter.ctx (by sorry)
+  let lhsOpStruct := lhsOp.get rewriter.ctx.val (by sorry)
   if lhsOpStruct.opType ≠ .arith .constant then
     return rewriter
 
   -- Get the rhs and check that it is a constant
-  let rhsValuePtr := op.getOperand rewriter.ctx 1 (by sorry) (by sorry)
+  let rhsValuePtr := op.getOperand rewriter.ctx.val 1 (by sorry) (by sorry)
   let rhsOp ← match rhsValuePtr with
   | ValuePtr.opResult rhsOpResultPtr => some rhsOpResultPtr.op
   | _ => none
-  let rhsOpStruct := rhsOp.get rewriter.ctx (by sorry)
+  let rhsOpStruct := rhsOp.get rewriter.ctx.val (by sorry)
   if rhsOpStruct.opType ≠ .arith .constant then
     return rewriter
 
   -- Sum both constant values
-  let lhsVal := (lhsOp.getProperties! rewriter.ctx (.arith .constant)).value.value
-  let rhsVal := (rhsOp.getProperties! rewriter.ctx (.arith .constant)).value.value
+  let lhsVal := (lhsOp.getProperties! rewriter.ctx.val (.arith .constant)).value.value
+  let rhsVal := (rhsOp.getProperties! rewriter.ctx.val (.arith .constant)).value.value
   let newVal := ArithConstantProperties.mk (IntegerAttr.mk (lhsVal + rhsVal) (IntegerType.mk 32))
   let (rewriter, newOp) ← rewriter.createOp (.arith .constant) #[IntegerType.mk 32] #[] #[] #[] newVal (some $ .before op) sorry sorry sorry sorry
-  let mut rewriter ← rewriter.replaceOp op newOp sorry sorry sorry
+  let mut rewriter ← rewriter.replaceOp op newOp sorry sorry sorry sorry sorry
 
-  if (lhsValuePtr.getFirstUse rewriter.ctx (by sorry)).isNone then
-    rewriter ← rewriter.eraseOp lhsOp sorry
-  if (rhsValuePtr.getFirstUse rewriter.ctx (by sorry)).isNone then
-    rewriter ← rewriter.eraseOp rhsOp sorry
+  if (lhsValuePtr.getFirstUse rewriter.ctx.val (by sorry)).isNone then
+    rewriter ← rewriter.eraseOp lhsOp sorry sorry sorry
+  if (rhsValuePtr.getFirstUse rewriter.ctx.val (by sorry)).isNone then
+    rewriter ← rewriter.eraseOp rhsOp sorry sorry sorry
   return rewriter
 
-def addIConstantFoldingLocal (ctx: IRContext OpCode) (op: OperationPtr) :
-    Option (IRContext OpCode × Option (Array OperationPtr × Array ValuePtr)) := do
+def addIConstantFoldingLocal (ctx: WfIRContext OpCode) (op: OperationPtr) :
+    Option (WfIRContext OpCode × Option (Array OperationPtr × Array ValuePtr)) := do
   -- Check that the operation is an `arith.addi` operation
-  let .arith .addi := op.getOpType ctx sorry
+  let .arith .addi := op.getOpType ctx.val sorry
     | some (ctx, none)
   -- Get the lhs and check that it is a constant
-  let lhsValuePtr := op.getOperand ctx 0 (by sorry) (by sorry)
+  let lhsValuePtr := op.getOperand ctx.val 0 (by sorry) (by sorry)
   let .opResult lhsOpResultPtr := lhsValuePtr
     | some (ctx, none)
   let lhsOp := lhsOpResultPtr.op
-  let lhsOpStruct := lhsOp.get ctx (by sorry)
+  let lhsOpStruct := lhsOp.get ctx.val (by sorry)
   let .arith .constant := lhsOpStruct.opType
     | some (ctx, none)
 
   -- Get the rhs and check that it is a constant
-  let rhsValuePtr := op.getOperand ctx 1 (by sorry) (by sorry)
+  let rhsValuePtr := op.getOperand ctx.val 1 (by sorry) (by sorry)
   let .opResult rhsOpResultPtr := rhsValuePtr
     | some (ctx, none)
   let rhsOp := rhsOpResultPtr.op
-  let rhsOpStruct := rhsOp.get ctx (by sorry)
+  let rhsOpStruct := rhsOp.get ctx.val (by sorry)
   let .arith .constant := rhsOpStruct.opType
     | some (ctx, none)
 
   -- Sum both constant values
-  let lhsVal := (lhsOp.getProperties! ctx (.arith .constant)).value.value
-  let rhsVal := (rhsOp.getProperties! ctx (.arith .constant)).value.value
+  let lhsVal := (lhsOp.getProperties! ctx.val (.arith .constant)).value.value
+  let rhsVal := (rhsOp.getProperties! ctx.val (.arith .constant)).value.value
   let newVal := ArithConstantProperties.mk (IntegerAttr.mk (lhsVal + rhsVal) (IntegerType.mk 32))
-  let (ctx, newOp) ← Rewriter.createOp ctx (.arith .constant) #[IntegerType.mk 32] #[] #[] #[] newVal none sorry sorry sorry sorry sorry
+  let (ctx, newOp) ← WfRewriter.createOp ctx (.arith .constant) #[IntegerType.mk 32] #[] #[] #[] newVal none sorry sorry sorry sorry
   return (ctx, some (#[newOp], #[newOp.getResult 0]))
 
 def addIZeroFolding (rewriter: PatternRewriter OpCode) (op: OperationPtr) : Option (PatternRewriter OpCode)   := do
-  if op.getOpType rewriter.ctx sorry ≠ .arith .addi then
+  if op.getOpType rewriter.ctx.val sorry ≠ .arith .addi then
     return rewriter
 
   -- Get the rhs and check that it is the constant 0
-  let rhsValuePtr := op.getOperand rewriter.ctx 1 (by sorry) (by sorry)
+  let rhsValuePtr := op.getOperand rewriter.ctx.val 1 (by sorry) (by sorry)
   let rhsOp ← match rhsValuePtr with
   | ValuePtr.opResult rhsOpResultPtr => some rhsOpResultPtr.op
   | _ => none
-  let rhsOpStruct := rhsOp.get rewriter.ctx (by sorry)
+  let rhsOpStruct := rhsOp.get rewriter.ctx.val (by sorry)
   if rhsOpStruct.opType ≠ .arith .constant then
     return rewriter
-  if (rhsOp.getProperties! rewriter.ctx (.arith .constant)).value.value ≠ 0 then
+  if (rhsOp.getProperties! rewriter.ctx.val (.arith .constant)).value.value ≠ 0 then
     return rewriter
 
   -- Get the lhs value
-  let lhsValuePtr := op.getOperand rewriter.ctx 0 (by sorry) (by sorry)
+  let lhsValuePtr := op.getOperand rewriter.ctx.val 0 (by sorry) (by sorry)
 
   let opValuePtr := op.getResult 0
   let mut rewriter ← rewriter.replaceValue opValuePtr lhsValuePtr sorry sorry
-  rewriter ← rewriter.eraseOp op sorry
+  rewriter ← rewriter.eraseOp op sorry sorry sorry
 
-  if (rhsValuePtr.getFirstUse rewriter.ctx (by sorry)).isNone then
-    rewriter ← rewriter.eraseOp rhsOp sorry
+  if (rhsValuePtr.getFirstUse rewriter.ctx.val (by sorry)).isNone then
+    rewriter ← rewriter.eraseOp rhsOp sorry sorry sorry
   return rewriter
 
 def mulITwoReduce (rewriter: PatternRewriter OpCode) (op: OperationPtr) : Option (PatternRewriter OpCode) := do
-  if op.getOpType rewriter.ctx sorry ≠ .arith .muli then
+  if op.getOpType rewriter.ctx.val sorry ≠ .arith .muli then
     return rewriter
 
   -- Get the rhs and check that it is the constant 2
-  let rhsValuePtr := op.getOperand rewriter.ctx 1 (by sorry) (by sorry)
+  let rhsValuePtr := op.getOperand rewriter.ctx.val 1 (by sorry) (by sorry)
   let rhsOp ← match rhsValuePtr with
   | ValuePtr.opResult rhsOpResultPtr => some rhsOpResultPtr.op
   | _ => none
-  let rhsOpStruct := rhsOp.get rewriter.ctx (by sorry)
+  let rhsOpStruct := rhsOp.get rewriter.ctx.val (by sorry)
   if rhsOpStruct.opType ≠ .arith .constant then
     return rewriter
-  if (rhsOp.getProperties! rewriter.ctx (.arith .constant)).value.value ≠ 2 then
+  if (rhsOp.getProperties! rewriter.ctx.val (.arith .constant)).value.value ≠ 2 then
     return rewriter
 
   -- Get the lhs value
-  let lhsValuePtr := op.getOperand rewriter.ctx 0 (by sorry) (by sorry)
+  let lhsValuePtr := op.getOperand rewriter.ctx.val 0 (by sorry) (by sorry)
 
   let (rewriter, newOp) ← rewriter.createOp (.arith .addi) #[IntegerType.mk 32] #[lhsValuePtr, lhsValuePtr] #[] #[] (NswNuwProperties.mk false false) (some $ .before op) sorry sorry sorry sorry
-  let mut rewriter ← rewriter.replaceOp op newOp sorry sorry sorry
+  let mut rewriter ← rewriter.replaceOp op newOp sorry sorry sorry sorry sorry
 
-  if (rhsValuePtr.getFirstUse rewriter.ctx (by sorry)).isNone then
-    rewriter ← rewriter.eraseOp rhsOp sorry
+  if (rhsValuePtr.getFirstUse rewriter.ctx.val (by sorry)).isNone then
+    rewriter ← rewriter.eraseOp rhsOp sorry sorry sorry
   return rewriter
 
 end Pattern
@@ -139,119 +139,120 @@ end Pattern
 -- applying the rewrites in custom locations
 namespace Custom
 
-abbrev Pattern := (IRContext OpCode) → OperationPtr → Option (IRContext OpCode)
+abbrev Pattern := (WfIRContext OpCode) → OperationPtr → Option (WfIRContext OpCode)
 
-def addIConstantFolding (ctx: IRContext OpCode) (op: OperationPtr) : Option (IRContext OpCode) := do
+def addIConstantFolding (ctx: WfIRContext OpCode) (op: OperationPtr) : Option (WfIRContext OpCode) := do
   -- Check that the operation is an arith.addi operation
-  if op.getOpType ctx sorry ≠ .arith .addi then
+  if op.getOpType ctx.val sorry ≠ .arith .addi then
     return ctx
 
   -- Get the lhs and check that it is a constant
-  let lhsValuePtr := op.getOperand ctx 0 (by sorry) (by sorry)
+  let lhsValuePtr := op.getOperand ctx.val 0 (by sorry) (by sorry)
   let lhsOp ← match lhsValuePtr with
   | ValuePtr.opResult lhsOpResultPtr => some lhsOpResultPtr.op
   | _ => none
-  let lhsOpStruct := lhsOp.get ctx (by sorry)
+  let lhsOpStruct := lhsOp.get ctx.val (by sorry)
   if lhsOpStruct.opType ≠ .arith .constant then
     return ctx
 
   -- Get the rhs and check that it is a constant
-  let rhsValuePtr := op.getOperand ctx 1 (by sorry) (by sorry)
+  let rhsValuePtr := op.getOperand ctx.val 1 (by sorry) (by sorry)
   let rhsOp ← match rhsValuePtr with
   | ValuePtr.opResult rhsOpResultPtr => some rhsOpResultPtr.op
   | _ => none
-  let rhsOpStruct := rhsOp.get ctx (by sorry)
+  let rhsOpStruct := rhsOp.get ctx.val (by sorry)
   if rhsOpStruct.opType ≠ .arith .constant then
     return ctx
 
   -- Sum both constant values
-  let lhsVal := (lhsOp.getProperties! ctx (.arith .constant)).value.value
-  let rhsVal := (rhsOp.getProperties! ctx (.arith .constant)).value.value
+  let lhsVal := (lhsOp.getProperties! ctx.val (.arith .constant)).value.value
+  let rhsVal := (rhsOp.getProperties! ctx.val (.arith .constant)).value.value
   let newVal := ArithConstantProperties.mk (IntegerAttr.mk (lhsVal + rhsVal) (IntegerType.mk 32))
-  let (ctx, newOp) ← Rewriter.createOp ctx (.arith .constant) #[IntegerType.mk 32] #[] #[] #[] newVal (some $ .before op) sorry sorry sorry sorry sorry
-  let mut ctx ← Rewriter.replaceOp? ctx op newOp sorry sorry sorry sorry
+  let (ctx, newOp) ← WfRewriter.createOp ctx (.arith .constant) #[IntegerType.mk 32] #[] #[] #[] newVal (some $ .before op) sorry sorry sorry sorry
+  let mut ctx ← WfRewriter.replaceOp? ctx op newOp sorry sorry sorry sorry sorry
 
-  if (lhsValuePtr.getFirstUse ctx (by sorry)).isNone then
-    ctx ← Rewriter.eraseOp ctx lhsOp sorry sorry
-  if (rhsValuePtr.getFirstUse ctx (by sorry)).isNone then
-    ctx ← Rewriter.eraseOp ctx rhsOp sorry sorry
+  if (lhsValuePtr.getFirstUse ctx.val (by sorry)).isNone then
+    ctx ← WfRewriter.eraseOp ctx lhsOp sorry sorry sorry
+  if (rhsValuePtr.getFirstUse ctx.val (by sorry)).isNone then
+    ctx ← WfRewriter.eraseOp ctx rhsOp sorry sorry sorry
   return ctx
 
-def addIZeroFolding (ctx: IRContext OpCode) (op: OperationPtr) : Option (IRContext OpCode) := do
-  if op.getOpType ctx sorry ≠ .arith .addi then
+def addIZeroFolding (ctx: WfIRContext OpCode) (op: OperationPtr) : Option (WfIRContext OpCode) := do
+  if op.getOpType ctx.val sorry ≠ .arith .addi then
     return ctx
 
   -- Get the rhs and check that it is the constant 0
-  let rhsValuePtr := op.getOperand ctx 1 (by sorry) (by sorry)
+  let rhsValuePtr := op.getOperand ctx.val 1 (by sorry) (by sorry)
   let rhsOp ← match rhsValuePtr with
   | ValuePtr.opResult rhsOpResultPtr => some rhsOpResultPtr.op
   | _ => none
-  let rhsOpStruct := rhsOp.get ctx (by sorry)
+  let rhsOpStruct := rhsOp.get ctx.val (by sorry)
   if rhsOpStruct.opType ≠ .arith .constant then
     return ctx
-  if (rhsOp.getProperties! ctx (.arith .constant)).value.value ≠ 0 then
+  if (rhsOp.getProperties! ctx.val (.arith .constant)).value.value ≠ 0 then
     return ctx
 
   -- Get the lhs value
-  let lhsValuePtr := op.getOperand ctx 0 (by sorry) (by sorry)
+  let lhsValuePtr := op.getOperand ctx.val 0 (by sorry) (by sorry)
 
   let oldVal := op.getResult 0
-  let mut ctx ← Rewriter.replaceValue? ctx oldVal lhsValuePtr sorry sorry sorry
-  ctx ← Rewriter.eraseOp ctx op sorry sorry
+  let mut ctx ← WfRewriter.replaceValue ctx oldVal lhsValuePtr sorry sorry
+  ctx ← WfRewriter.eraseOp ctx op sorry sorry sorry
 
-  if (rhsValuePtr.getFirstUse ctx (by sorry)).isNone then
-    ctx ← Rewriter.eraseOp ctx rhsOp sorry sorry
+  if (rhsValuePtr.getFirstUse ctx.val (by sorry)).isNone then
+    ctx ← WfRewriter.eraseOp ctx rhsOp sorry sorry sorry
   return ctx
 
-def mulITwoReduce (ctx: IRContext OpCode) (op: OperationPtr) : Option (IRContext OpCode) := do
-  if op.getOpType ctx sorry ≠ .arith .muli then
+def mulITwoReduce (ctx: WfIRContext OpCode) (op: OperationPtr) : Option (WfIRContext OpCode) := do
+  if op.getOpType ctx.val sorry ≠ .arith .muli then
     return ctx
 
   -- Get the rhs and check that it is the constant 2
-  let rhsValuePtr := op.getOperand ctx 1 (by sorry) (by sorry)
+  let rhsValuePtr := op.getOperand ctx.val 1 (by sorry) (by sorry)
   let rhsOp ← match rhsValuePtr with
   | ValuePtr.opResult rhsOpResultPtr => some rhsOpResultPtr.op
   | _ => none
-  let rhsOpStruct := rhsOp.get ctx (by sorry)
+  let rhsOpStruct := rhsOp.get ctx.val (by sorry)
   if rhsOpStruct.opType ≠ .arith .constant then
     return ctx
-  if (rhsOp.getProperties! ctx (.arith .constant)).value.value ≠ 2 then
+  if (rhsOp.getProperties! ctx.val (.arith .constant)).value.value ≠ 2 then
     return ctx
 
   -- Get the lhs value
-  let lhsValuePtr := op.getOperand ctx 0 (by sorry) (by sorry)
+  let lhsValuePtr := op.getOperand ctx.val 0 (by sorry) (by sorry)
 
-  let (ctx, newOp) ← Rewriter.createOp ctx (.arith .addi) #[IntegerType.mk 32] #[lhsValuePtr, lhsValuePtr] #[] #[] (NswNuwProperties.mk false false) (some $ .before op) sorry sorry sorry sorry sorry
-  let mut ctx ← Rewriter.replaceOp? ctx op newOp sorry sorry sorry sorry
+  let (ctx, newOp) ← WfRewriter.createOp ctx (.arith .addi) #[IntegerType.mk 32] #[lhsValuePtr, lhsValuePtr] #[] #[] (NswNuwProperties.mk false false) (some $ .before op) sorry sorry sorry sorry
+  let mut ctx ← WfRewriter.replaceOp? ctx op newOp sorry sorry sorry sorry sorry
 
-  if (rhsValuePtr.getFirstUse ctx (by sorry)).isNone then
-    ctx ← Rewriter.eraseOp ctx rhsOp sorry sorry
+  if (rhsValuePtr.getFirstUse ctx.val (by sorry)).isNone then
+    ctx ← WfRewriter.eraseOp ctx rhsOp sorry sorry sorry
   return ctx
 
 -- Rewrites the first instance of an opcode in the program with the given pattern,
 -- within a program consisting of one region/block
-def rewriteFirst (ctx: IRContext OpCode) (topOp : OperationPtr) (opcode: OpCode) (rewrite: Pattern) : Option (IRContext OpCode) := do
-  let region := topOp.getRegion! ctx 0
-  let block := (region.get ctx (by sorry)).firstBlock.get!
-  let mut op ← (block.get! ctx).firstOp
+def rewriteFirst (ctx: WfIRContext OpCode) (topOp : OperationPtr) (opcode: OpCode) (rewrite: Pattern)
+    : Option (WfIRContext OpCode) := do
+  let region := topOp.getRegion! ctx.val 0
+  let block := (region.get ctx.val (by sorry)).firstBlock.get!
+  let mut op ← (block.get! ctx.val).firstOp
 
   while op.getOpType ctx sorry ≠ opcode do
-    op ← (op.get! ctx).next
+    op ← (op.get! ctx.val).next
 
   rewrite ctx op
 
-def rewriteFirstAddI (ctx: IRContext OpCode) (topOp : OperationPtr) (rewrite: Pattern) : Option (IRContext OpCode) :=
+def rewriteFirstAddI (ctx: WfIRContext OpCode) (topOp : OperationPtr) (rewrite: Pattern) : Option (WfIRContext OpCode) :=
   rewriteFirst ctx topOp (.arith .addi) rewrite
 
-def rewriteForwards (ctx: IRContext OpCode) (topOp : OperationPtr) (rewrite: Pattern) : Option (IRContext OpCode) := do
-  let region := topOp.getRegion! ctx 0
-  let block := (region.get ctx (by sorry)).firstBlock.get!
+def rewriteForwards (ctx: WfIRContext OpCode) (topOp : OperationPtr) (rewrite: Pattern) : Option (WfIRContext OpCode) := do
+  let region := topOp.getRegion! ctx.val 0
+  let block := (region.get ctx.val (by sorry)).firstBlock.get!
 
-  let mut maybeOp := (block.get! ctx).firstOp
+  let mut maybeOp := (block.get! ctx.val).firstOp
   let mut ctx := ctx
   while h : maybeOp.isSome do
     let op := maybeOp.get h
-    let next := (op.get! ctx).next
+    let next := (op.get! ctx.val).next
     -- TODO: This should be work but for some reason is not unique
     -- ctx := dbgTraceIfShared "rewriteForwards" ctx
     -- ctx ← rewrite ctx op
@@ -263,10 +264,10 @@ end Custom
 
 namespace Program
 
-def empty : Option (IRContext OpCode × OperationPtr × InsertPoint) := do
-  let (ctx, topLevelOp) ← IRContext.create OpCode
-  let region := topLevelOp.getRegion! ctx 0
-  let block := (region.get ctx (by sorry)).firstBlock.get!
+def empty : Option (WfIRContext OpCode × OperationPtr × InsertPoint) := do
+  let (ctx, topLevelOp) ← WfIRContext.create OpCode
+  let region := topLevelOp.getRegion! ctx.val 0
+  let block := (region.get ctx.val (by sorry)).firstBlock.get!
   let insertPoint := InsertPoint.atEnd block
   (ctx, topLevelOp, insertPoint)
 
@@ -279,31 +280,31 @@ def empty : Option (IRContext OpCode × OperationPtr × InsertPoint) := do
 --   %3 = arith.constant [inc] : u64
 --   %4 = [opcode] %2, %3 : u64
 --   ...
-def constFoldTree (opcode: OpCode) (prop : propertiesOf opcode) (size pc: Nat) (root inc: Int) : Option (IRContext OpCode × OperationPtr) := do
+def constFoldTree (opcode: OpCode) (prop : propertiesOf opcode) (size pc: Nat) (root inc: Int) : Option (WfIRContext OpCode × OperationPtr) := do
   let root := ArithConstantProperties.mk (IntegerAttr.mk root (IntegerType.mk 32))
   let inc := ArithConstantProperties.mk (IntegerAttr.mk inc (IntegerType.mk 32))
   let (gctx, topOp, insertPoint) ← empty
-  let mut (gctx, gacc) ← Rewriter.createOp gctx (.arith .constant) #[IntegerType.mk 32] #[] #[] #[] root insertPoint sorry sorry sorry sorry sorry
+  let mut (gctx, gacc) ← WfRewriter.createOp gctx (.arith .constant) #[IntegerType.mk 32] #[] #[] #[] root insertPoint sorry sorry sorry sorry
   for i in [0:size] do
     let ⟨thisOp, prop⟩ : (op : OpCode) × propertiesOf op := if (i % 100 < pc) then ⟨opcode, prop⟩ else ⟨.arith .andi, ()⟩
     let (ctx, acc) := (gctx, gacc)
-    let (ctx, rhsOp) ← Rewriter.createOp ctx (.arith .constant) #[IntegerType.mk 32] #[] #[] #[] inc insertPoint sorry sorry sorry sorry sorry
+    let (ctx, rhsOp) ← WfRewriter.createOp ctx (.arith .constant) #[IntegerType.mk 32] #[] #[] #[] inc insertPoint sorry sorry sorry sorry
     let lhsVal := acc.getResult 0
     let rhsVal := rhsOp.getResult 0
-    let (ctx, acc) ← Rewriter.createOp ctx thisOp #[IntegerType.mk 32] #[lhsVal, rhsVal] #[] #[] prop insertPoint sorry sorry sorry sorry sorry
+    let (ctx, acc) ← WfRewriter.createOp ctx thisOp #[IntegerType.mk 32] #[lhsVal, rhsVal] #[] #[] prop insertPoint sorry sorry sorry sorry
     (gctx, gacc) := (ctx, acc)
 
   let accRes := gacc.getResult 0
-  let (ctx, op) ← Rewriter.createOp gctx (.test .test) #[] #[accRes] #[] #[] () insertPoint sorry sorry sorry sorry sorry
+  let (ctx, op) ← WfRewriter.createOp gctx (.test .test) #[] #[accRes] #[] #[] () insertPoint sorry sorry sorry sorry
   (ctx, topOp)
 
-def addZeroTree (size pc: Nat) : Option (IRContext OpCode × OperationPtr) :=
+def addZeroTree (size pc: Nat) : Option (WfIRContext OpCode × OperationPtr) :=
   constFoldTree (.arith .addi) (NswNuwProperties.mk false false) size pc 42 0
 
-def addOneTree (size pc: Nat) : Option (IRContext OpCode × OperationPtr) :=
+def addOneTree (size pc: Nat) : Option (WfIRContext OpCode × OperationPtr) :=
   constFoldTree (.arith .addi) (NswNuwProperties.mk false false) size pc 42 1
 
-def mulTwoTree (size pc: Nat) : Option (IRContext OpCode × OperationPtr) :=
+def mulTwoTree (size pc: Nat) : Option (WfIRContext OpCode × OperationPtr) :=
   constFoldTree (.arith .muli) (NswNuwProperties.mk false false) size pc 42 2
 
 
@@ -314,12 +315,12 @@ def mulTwoTree (size pc: Nat) : Option (IRContext OpCode × OperationPtr) :=
 --   %2 = [opcode] %0, %reuse : u64
 --   %3 = [opcode] %2, %reuse : u64
 --   ...
-def constReuseTree (opcode: OpCode) (prop : propertiesOf opcode) (size pc: Nat) (root inc: Int) : Option (IRContext OpCode × OperationPtr) := do
+def constReuseTree (opcode: OpCode) (prop : propertiesOf opcode) (size pc: Nat) (root inc: Int) : Option (WfIRContext OpCode × OperationPtr) := do
   let root := ArithConstantProperties.mk (IntegerAttr.mk root (IntegerType.mk 32))
   let inc := ArithConstantProperties.mk (IntegerAttr.mk inc (IntegerType.mk 32))
   let (ctx, topOp, insertPoint) ← empty
-  let (ctx, acc) ← Rewriter.createOp ctx (.arith .constant) #[IntegerType.mk 32] #[] #[] #[] root insertPoint sorry sorry sorry sorry sorry
-  let (ctx, reuse) ← Rewriter.createOp ctx (.arith .constant) #[IntegerType.mk 32] #[] #[] #[] inc insertPoint sorry sorry sorry sorry sorry
+  let (ctx, acc) ← WfRewriter.createOp ctx (.arith .constant) #[IntegerType.mk 32] #[] #[] #[] root insertPoint sorry sorry sorry sorry
+  let (ctx, reuse) ← WfRewriter.createOp ctx (.arith .constant) #[IntegerType.mk 32] #[] #[] #[] inc insertPoint sorry sorry sorry sorry
 
   let mut (gctx, gacc) := (ctx, acc)
   for i in [0:size] do
@@ -328,15 +329,15 @@ def constReuseTree (opcode: OpCode) (prop : propertiesOf opcode) (size pc: Nat) 
     let (ctx, acc) := (gctx, gacc)
     let lhsVal := acc.getResult 0
     let rhsVal := reuse.getResult 0
-    let (ctx, acc) ← Rewriter.createOp ctx thisOp #[IntegerType.mk 32] #[lhsVal, rhsVal] #[] #[] prop insertPoint sorry sorry sorry sorry sorry
+    let (ctx, acc) ← WfRewriter.createOp ctx thisOp #[IntegerType.mk 32] #[lhsVal, rhsVal] #[] #[] prop insertPoint sorry sorry sorry sorry
     (gctx, gacc) := (ctx, acc)
   let (ctx, acc) := (gctx, gacc)
 
   let accRes := acc.getResult 0
-  let (ctx, op) ← Rewriter.createOp ctx (.test .test) #[] #[accRes] #[] #[] () insertPoint sorry sorry sorry sorry sorry
+  let (ctx, op) ← WfRewriter.createOp ctx (.test .test) #[] #[accRes] #[] #[] () insertPoint sorry sorry sorry sorry
   (ctx, topOp)
 
-def addZeroReuseTree (size pc: Nat) : Option (IRContext OpCode × OperationPtr) :=
+def addZeroReuseTree (size pc: Nat) : Option (WfIRContext OpCode × OperationPtr) :=
   constReuseTree (.arith .addi) (NswNuwProperties.mk false false) size pc 42 0
 
 -- Create a program that looks like:
@@ -348,15 +349,15 @@ def addZeroReuseTree (size pc: Nat) : Option (IRContext OpCode × OperationPtr) 
 --   %4 = [opcode] %3, %reuse : u64
 --   %5 = [opcode] %4, %reuse : u64
 --   ...
-def constLotsOfReuseTree (opcode: OpCode) (prop : propertiesOf opcode) (size pc: Nat) (lhs rhs: Int) : Option (IRContext OpCode × OperationPtr) := do
+def constLotsOfReuseTree (opcode: OpCode) (prop : propertiesOf opcode) (size pc: Nat) (lhs rhs: Int) : Option (WfIRContext OpCode × OperationPtr) := do
   let lhs := ArithConstantProperties.mk (IntegerAttr.mk lhs (IntegerType.mk 32))
   let rhs := ArithConstantProperties.mk (IntegerAttr.mk rhs (IntegerType.mk 32))
   let (ctx, topOp, insertPoint) ← empty
-  let (ctx, lhsOp) ← Rewriter.createOp ctx (.arith .constant) #[IntegerType.mk 32] #[] #[] #[] lhs insertPoint sorry sorry sorry sorry sorry
-  let (ctx, rhsOp) ← Rewriter.createOp ctx (.arith .constant) #[IntegerType.mk 32] #[] #[] #[] rhs insertPoint sorry sorry sorry sorry sorry
+  let (ctx, lhsOp) ← WfRewriter.createOp ctx (.arith .constant) #[IntegerType.mk 32] #[] #[] #[] lhs insertPoint sorry sorry sorry sorry
+  let (ctx, rhsOp) ← WfRewriter.createOp ctx (.arith .constant) #[IntegerType.mk 32] #[] #[] #[] rhs insertPoint sorry sorry sorry sorry
   let lhsVal := lhsOp.getResult 0
   let rhsVal := rhsOp.getResult 0
-  let (ctx, reuse) ← Rewriter.createOp ctx opcode #[IntegerType.mk 32] #[lhsVal, rhsVal] #[] #[] prop insertPoint sorry sorry sorry sorry sorry
+  let (ctx, reuse) ← WfRewriter.createOp ctx opcode #[IntegerType.mk 32] #[lhsVal, rhsVal] #[] #[] prop insertPoint sorry sorry sorry sorry
 
   let mut (gctx, gacc) := (ctx, reuse)
   for i in [0:size] do
@@ -365,23 +366,23 @@ def constLotsOfReuseTree (opcode: OpCode) (prop : propertiesOf opcode) (size pc:
     let (ctx, acc) := (gctx, gacc)
     let lhsVal := acc.getResult 0
     let rhsVal := reuse.getResult 0
-    let (ctx, acc) ← Rewriter.createOp ctx thisOp #[IntegerType.mk 32] #[lhsVal, rhsVal] #[] #[] prop insertPoint sorry sorry sorry sorry sorry
+    let (ctx, acc) ← WfRewriter.createOp ctx thisOp #[IntegerType.mk 32] #[lhsVal, rhsVal] #[] #[] prop insertPoint sorry sorry sorry sorry
     (gctx, gacc) := (ctx, acc)
   let (ctx, acc) := (gctx, gacc)
 
   let accRes := acc.getResult 0
-  let (ctx, op) ← Rewriter.createOp ctx (.test .test) #[] #[accRes] #[] #[] () insertPoint sorry sorry sorry sorry sorry
+  let (ctx, op) ← WfRewriter.createOp ctx (.test .test) #[] #[accRes] #[] #[] () insertPoint sorry sorry sorry sorry
   (ctx, topOp)
 
-def addZeroLotsOfReuseTree (size pc: Nat) : Option (IRContext OpCode × OperationPtr) :=
+def addZeroLotsOfReuseTree (size pc: Nat) : Option (WfIRContext OpCode × OperationPtr) :=
   constLotsOfReuseTree (.arith .addi) (NswNuwProperties.mk false false) size pc 42 0
 
 end Program
 
-def rewriteWorklist (program: IRContext OpCode) (topOp : OperationPtr) (rewriter: RewritePattern OpCode) : Option (IRContext OpCode):=
-  RewritePattern.applyInContext rewriter program sorry
+def rewriteWorklist (program: WfIRContext OpCode) (_topOp : OperationPtr) (rewriter: RewritePattern OpCode) : Option (WfIRContext OpCode):=
+  RewritePattern.applyInContext rewriter program
 
-def print (program: Option (IRContext OpCode × OperationPtr)) : IO Unit := do
+def print (program: Option (WfIRContext OpCode × OperationPtr)) : IO Unit := do
   if let some (ctx, topOp) := program then
     Printer.printModule ctx topOp
 
@@ -394,17 +395,17 @@ def time {α : Type} (name: String) (f: Unit → IO α) (quiet: Bool) : IO α :=
     IO.println s!"{name} time (s): {elapsedTime.toFloat / 1000000000}"
   return res
 
-def run {pattern : Type} (size pc: Nat) (create: Nat → Nat → Option (IRContext OpCode × OperationPtr))
-    (rewriteDriver: IRContext OpCode → OperationPtr → pattern → Option (IRContext OpCode))
+def run {pattern : Type} (size pc: Nat) (create: Nat → Nat → Option (WfIRContext OpCode × OperationPtr))
+    (rewriteDriver: WfIRContext OpCode → OperationPtr → pattern → Option (WfIRContext OpCode))
     (rewritePattern: pattern)
-    (doPrint: Bool) (quiet: Bool := false) : OptionT IO (IRContext OpCode × OperationPtr) := do
+    (doPrint: Bool) (quiet: Bool := false) : OptionT IO (WfIRContext OpCode × OperationPtr) := do
   let (ctx, topOp) ← time "create" (fun () => return create size pc) quiet
   let ctx ← time "rewrite" (fun () => return rewriteDriver ctx topOp rewritePattern) quiet
   if doPrint && !quiet then
     print (ctx, topOp)
   return (ctx, topOp)
 
-def runBenchmarkWithResult (benchmark: String) (n pc: Nat) (quiet: Bool := false) : OptionT IO (IRContext OpCode × OperationPtr) :=
+def runBenchmarkWithResult (benchmark: String) (n pc: Nat) (quiet: Bool := false) : OptionT IO (WfIRContext OpCode × OperationPtr) :=
   open Program in
   open Custom in
 
