Veir/Passes/CastsReconciliation/Reconciliation.lean
@@ -12,27 +12,27 @@ set_option warn.sorry false in
 def reconcileRegistersPairingCast (rewriter : PatternRewriter OpCode) (op : OperationPtr) :
     Option (PatternRewriter OpCode) := do
   let some cast := matchCastOp op rewriter.ctx | return rewriter
-  let input := op.getOperand! rewriter.ctx 0
-  let inputType := input.getType! rewriter.ctx
-  let resultType := ((op.getResult 0).get! rewriter.ctx).type
+  let input := op.getOperand! rewriter.ctx.val 0
+  let inputType := input.getType! rewriter.ctx.val
+  let resultType := ((op.getResult 0).get! rewriter.ctx.val).type
   /- Only consider casting between `!reg` and `i64` types-/
   if ¬ (inputType = RegisterType.mk ∧ resultType = IntegerType.mk 64) ∧
        ¬ (inputType = IntegerType.mk 64 ∧ resultType = RegisterType.mk) then return rewriter
   /- If the operand's parent is a cast operation -/
   let .opResult op' := input | return rewriter
   let some cast := matchCastOp op'.op rewriter.ctx | return rewriter
-  let parentInput := (op'.op.getOperand! rewriter.ctx 0)
+  let parentInput := (op'.op.getOperand! rewriter.ctx.val 0)
   /- And the result's type coincides with the parent operation operand's type -/
-  let parentInputType := parentInput.getType! rewriter.ctx
+  let parentInputType := parentInput.getType! rewriter.ctx.val
   if resultType ≠ parentInputType then return rewriter
   /- Replace the initial operation's output with the parent operations input -/
   let rewriter ← rewriter.replaceValue (op.getResult 0) parentInput sorry sorry
   /- Erase the redundant cast operation -/
-  let rewriter ← rewriter.eraseOp op sorry
+  let rewriter ← rewriter.eraseOp op sorry sorry sorry
   /- If unused and side-effect-free, erase the parent cast operation as well.
     These need to be erased in this order, otherwise the parent operation will always be used. -/
-  if ¬ op'.op.hasUses! rewriter.ctx && hasSideEffects rewriter op'.op then
-    rewriter.eraseOp op'.op sorry
+  if ¬ op'.op.hasUses! rewriter.ctx.val && hasSideEffects rewriter op'.op then
+    rewriter.eraseOp op'.op sorry sorry sorry
   else
     return rewriter
 
@@ -50,53 +50,51 @@ def reconcileRegistersPairingCast (rewriter : PatternRewriter OpCode) (op : Oper
 set_option warn.sorry false in
 def reconcileIntegersPairingCast (rewriter : PatternRewriter OpCode) (op : OperationPtr) :
     Option (PatternRewriter OpCode) := do
-  let some cast := matchCastOp op rewriter.ctx | return rewriter
-  let input := op.getOperand! rewriter.ctx 0
-  let inputType := input.getType! rewriter.ctx
-  let resultType := ((op.getResult 0).get! rewriter.ctx).type
+  let some cast := matchCastOp op rewriter.ctx.val | return rewriter
+  let input := op.getOperand! rewriter.ctx.val 0
+  let inputType := input.getType! rewriter.ctx.val
+  let resultType := ((op.getResult 0).get! rewriter.ctx.val).type
   /- Only consider casting between `!reg` and `i64` types-/
-  let resultType := ((op.getResult 0).get! rewriter.ctx).type
+  let resultType := ((op.getResult 0).get! rewriter.ctx.val).type
   let IntegerType.mk bwRes := resultType | return rewriter
   let IntegerType.mk bwIn := inputType | return rewriter
   if bwIn ≤ bwRes then return rewriter
   /- If the operand's parent is a cast operation -/
   let .opResult op' := input | return rewriter
-  let some cast := matchCastOp op'.op rewriter.ctx | return rewriter
-  let parentInput := (op'.op.getOperand! rewriter.ctx 0)
+  let some cast := matchCastOp op'.op rewriter.ctx.val | return rewriter
+  let parentInput := (op'.op.getOperand! rewriter.ctx.val 0)
   /- And the result's type coincides with the parent operation operand's type -/
-  let parentInputType := parentInput.getType! rewriter.ctx
+  let parentInputType := parentInput.getType! rewriter.ctx.val
   if resultType ≠ parentInputType then return rewriter
   /- Replace the initial operation's output with the parent operations input -/
   let rewriter ← rewriter.replaceValue (op.getResult 0) parentInput sorry sorry
   /- Erase the redundant cast operation -/
-  let rewriter ← rewriter.eraseOp op sorry
+  let rewriter ← rewriter.eraseOp op sorry sorry sorry
   /- If unused and side-effect-free, erase the parent cast operation as well.
     These need to be erased in this order, otherwise the parent operation will always be used. -/
-  if ¬ op'.op.hasUses! rewriter.ctx && hasSideEffects rewriter op'.op then
-    rewriter.eraseOp op'.op sorry
+  if ¬ op'.op.hasUses! rewriter.ctx.val && hasSideEffects rewriter op'.op then
+    rewriter.eraseOp op'.op sorry sorry sorry
   else
     return rewriter
 
 set_option warn.sorry false in
 def reconcileIdentityCast (rewriter : PatternRewriter OpCode) (op : OperationPtr) :
     Option (PatternRewriter OpCode) := do
-  let some cast := matchCastOp op rewriter.ctx | return rewriter
+  let some cast := matchCastOp op rewriter.ctx.val | return rewriter
   /- get the input and output types -/
-  let input := op.getOperand! rewriter.ctx 0
-  let inputType := input.getType! rewriter.ctx
-  let resultType := ((op.getResult 0).get! rewriter.ctx).type
+  let input := op.getOperand! rewriter.ctx.val 0
+  let inputType := input.getType! rewriter.ctx.val
+  let resultType := ((op.getResult 0).get! rewriter.ctx.val).type
   if inputType ≠ resultType then return rewriter
   let rewriter ← rewriter.replaceValue (op.getResult 0) input sorry sorry
-  rewriter.eraseOp op sorry
+  rewriter.eraseOp op sorry sorry sorry
 
-set_option warn.sorry false in
-def CastReconcilePass.impl (ctx : { ctx' : IRContext OpCode // ctx'.WellFormed }) (op : OperationPtr)
-    (_ : op.InBounds ctx.val) :
-    ExceptT String IO { ctx' : IRContext OpCode // ctx'.WellFormed } := do
+def CastReconcilePass.impl (ctx : WfIRContext OpCode) (op : OperationPtr) (_ : op.InBounds ctx.val) :
+    ExceptT String IO (WfIRContext OpCode) := do
   let pattern := RewritePattern.GreedyRewritePattern #[reconcileIntegersPairingCast, reconcileRegistersPairingCast, reconcileIdentityCast]
-  match RewritePattern.applyInContext pattern ctx ctx.property.inBounds with
+  match RewritePattern.applyInContext pattern ctx with
   | none => throw "Error while applying cast reconciliation"
-  | some ctx => pure ⟨ctx, sorry⟩
+  | some ctx => pure ctx
 
 public def CastReconcilePass : Pass OpCode :=
   { name := "reconcile-cast"
